\begin{questions}

\question Find the closed formula for each of the following sequences by relating them to a well know sequence.  Assume the first term given is $a_1$.
\begin{parts}
  \part $2, 5, 10, 17, 26, \ldots$
  \part $0, 2, 5, 9, 14, 20, \ldots$
  \part $8, 12, 17, 23, 30,\ldots$
  \part $1, 5, 23, 119, 719,\ldots$
\end{parts}

	\begin{answer}
		\begin{parts}
		%$2, 5, 10, 17, 26, \ldots$
		  \part $a_n = n^2 + 1$
		%   $0, 2, 5, 9, 14, 20, \ldots$
		  \part $a_n = \frac{n(n+1)}{2} - 1$
		%   $8, 12, 17, 23, 30,\ldots$
		  \part $a_n = \frac{(n+2)(n+3)}{2} + 2$
		%   $1, 5, 23, 119, 719,\ldots$
		  \part $a_n = (n+1)! - 1$ (where $n! = 1 \cdot 2 \cdot 3 \cdots n$)
		\end{parts}
	\end{answer}
	
	
	

\question The Fibonacci sequence is $0, 1, 1, 2, 3, 5, 8, 13, \ldots$ (where $F_0 = 0$).
\begin{parts}
  \part Give the recursive definition for the sequence.
  \part Write out the first few terms of the sequence of partial sums.  
  \part Give a closed formula for the sequence of partial sums in terms of $F_n$  (for example, you might say $F_0 + F_1 + \cdots + F_n = 3F_{n-1}^2 + n$, although that is definitely not correct).
\end{parts}

	\begin{answer}
		\begin{parts}
		%Give the recursive definition for the sequence.
		  \part $F_n = F_{n-1} + F_{n-2}$ with $F_0 = 0$ and $F_1 = 1$.
		%   Write out the first few terms of the sequence of partial sums. 
		  \part  $0, 1, 2, 4, 7, 12, 20, \ldots$
		  %Give a closed formula for the sequence of partial sums in terms of $F_n$  (for example, you might say $F_0 + F_1 + \cdots + F_n = 3F_{n-1}^2 + n$, although that is definitely not correct).
		  \part $F_0 + F_1 + \cdots + F_n = F_{n+2} - 1$ 
		\end{parts}
	\end{answer}
	
	
	


\question Write out the first few terms of the sequence given by $a_1 = 3$; $a_n = 2a_{n-1} + 4$.  Then find a recursive definition for the sequence $10, 24, 52, 108, \ldots$.

	\begin{answer}
		$3, 10, 24, 52, 108,\ldots$.  The recursive definition for $10, 24, 52, \ldots$ is $a_n = 2a_{n-1} + 4$ with $a_1 = 10$.
	\end{answer}
	
	
	


\question Write out the first few terms of the sequence given by $a_n = n^2 - 3n + 1$.  Then find a closed formula for the sequence (starting with $a_1$) $0, 2, 6, 12, 20, \ldots$.

	\begin{answer}
		$-1, -1, 1, 5, 11, 19,\ldots$  Thus the sequence $0, 2, 6, 12, 20,\ldots$ has closed formula $a_n = (n+1)^2 - 3(n+1) + 2$.
	\end{answer}
	
\end{questions}