<?xml version="1.0" encoding="UTF-8"?>
<exercises xmlns:xi="http://www.w3.org/2001/XInclude" xml:id="exercises_sec-logic" permid="Shv">

  <exercise permid="iCQ">
    <statement>
      <p permid="JTc">
        Consider the statement about a party,
        <q>If it's your birthday or there will be cake,
        then there will be cake.</q>

        <ol permid="HPu">
          <li permid="lbX">
            <p permid="bmM">
              Translate the above statement into symbols.
              Clearly state which statement is <m>P</m> and which is <m>Q</m>.
            </p>
          </li>

          <li permid="Rjg">
            <p permid="HtV">
              Make a truth table for the statement.
            </p>
          </li>

          <li permid="xqp">
            <p permid="nBe">
              Assuming the statement is true, what
              (if anything)
              can you conclude if there will be cake?
            </p>
          </li>

          <li permid="dxy">
            <p permid="TIn">
              Assuming the statement is true, what
              (if anything)
              can you conclude if there will not be cake?
            </p>
          </li>

          <li permid="JEH">
            <p permid="zPw">
              Suppose you found out that the statement was a lie.
              What can you conclude?
            </p>
          </li>
        </ol>
      </p>
    </statement>
    <solution permid="Bqo">
      <p permid="bWG">
        <ol permid="jmK">
          <li permid="pLQ">
            <m>P</m>: it's your birthday; <m>Q</m>:
            there will be cake. <m>(P \vee Q) \imp Q</m>
          </li>

          <li permid="VSZ">
            <p permid="fWF">
              Hint: you should get three T's and one F.
            </p>
          </li>

          <li permid="Cai">
            <p permid="MdO">
              Only that there will be cake.
            </p>
          </li>

          <li permid="ihr">
            <p permid="skX">
              It's NOT your birthday!
            </p>
          </li>

          <li permid="OoA">
            <p permid="Ysg">
              It's your birthday, but the cake is a lie.
            </p>
          </li>
        </ol>
      </p>
    </solution>
  </exercise>

  <exercise permid="OJZ">
    <statement>
      <p permid="qal">
        Make a truth table for the statement <m>(P \vee Q) \imp (P \wedge Q)</m>.
      </p>
    </statement>
    <solution permid="hxx">
      <sidebyside permid="lxw">

        <tabular halign="center" permid="Vcb">
          <col right="minor"/>
          <col right="medium"/>
          <col/>
          <row bottom="minor">
            <cell><m>P</m></cell>
            <cell><m>Q</m></cell>
            <cell><m>(P \vee Q) \imp (P \wedge Q)</m></cell>
          </row>
          <row>
            <cell>T</cell>
            <cell>T</cell>
            <cell>T</cell>
          </row>
          <row>
            <cell>T</cell>
            <cell>F</cell>
            <cell>F</cell>
          </row>
          <row>
            <cell>F</cell>
            <cell>T</cell>
            <cell>F</cell>
          </row>
          <row>
            <cell>F</cell>
            <cell>F</cell>
            <cell>T</cell>
          </row>
        </tabular>

      </sidebyside>
    </solution>
  </exercise>

  <exercise permid="uRi">
    <statement>
      <p permid="Whu">
        Make a truth table for the statement <m>\neg P \wedge (Q \imp P)</m>.
        What can you conclude about <m>P</m> and <m>Q</m> if you know the statement is true?
      </p>
    </statement>
    <solution permid="NEG">
      <sidebyside permid="REF">

        <tabular halign="center" permid="Bjk">
          <col right="minor"/>
          <col right="medium"/>
          <col/>
          <row bottom="minor">
            <cell><m>P</m></cell>
            <cell><m>Q</m></cell>
            <cell><m>\neg P \wedge (Q \imp P)</m></cell>
          </row>
          <row>
            <cell>T</cell>
            <cell>T</cell>
            <cell>F</cell>
          </row>
          <row>
            <cell>T</cell>
            <cell>F</cell>
            <cell>F</cell>
          </row>
          <row>
            <cell>F</cell>
            <cell>T</cell>
            <cell>F</cell>
          </row>
          <row>
            <cell>F</cell>
            <cell>F</cell>
            <cell>T</cell>
          </row>
        </tabular>

      </sidebyside>

      <p permid="IdP">
        If the statement is true, then both <m>P</m> and <m>Q</m> are false.
      </p>
    </solution>
  </exercise>

  <exercise permid="aYr">
    <statement>
      <p permid="CoD">
        Make a truth table for the statement <m>\neg P \imp (Q \wedge R)</m>.
      </p>
    </statement>
    <hint permid="tLP">
      <p permid="MNI">
        Like above, only now you will need 8 rows instead of just 4.
      </p>
    </hint>
  </exercise>
  
  <exercise permid="HfA">
    <statement>
      <p permid="ivM">
        Geoff Poshingten is out at a fancy pizza joint,
        and decides to order a calzone.
        When the waiter asks what he would like in it, he replies,
        <q>I want either pepperoni or sausage.
        Also, if I have sausage, then I must also include quail.
        Oh, and if I have pepperoni or quail then I must also have ricotta cheese.</q>

        <ol permid="nWD">
          <li permid="uvJ">
            <p permid="Ezp">
              Translate Geoff's order into logical symbols.
            </p>
          </li>

          <li permid="aCS">
            <p permid="kGy">
              The waiter knows that Geoff is either a liar or a truth-teller
              (so either everything he says is false, or everything is true).
              Which is it?
            </p>
          </li>

          <li permid="GKb">
            <p permid="QNH">
              What, if anything,
              can the waiter conclude about the ingredients in Geoff's desired calzone?
            </p>
          </li>
        </ol>
      </p>
    </statement>
    <hint permid="ZSY">
      <p permid="sUR">
        You should write down three statements using the symbols <m>P, Q, R, S</m>.  If Geoff is a truth-teller, then all three statements would be true.  If he was a liar, then all three statements would be false.  But in either case, we don't yet know whether the four atomic statements are true or false, since he hasn't said them by themselves. 
      </p>
      
      <p permid="Zca">
        A truth table might help, although is probably not entirely necessary.
      </p>
    </hint>
  </exercise>

  <exercise permid="nmJ">
    <statement>
      <p permid="OCV">
        Determine whether the following two statements are logically equivalent:
        <m>\neg(P \imp Q)</m> and <m>P \wedge \neg Q</m>.
        Explain how you know you are correct.
      </p>
    </statement>
    <solution permid="Gah">
      <p permid="okY">
        Make a truth table for each and compare.
        The statements are logically equivalent.
      </p>
    </solution>
  </exercise>

  <exercise permid="TtS">
    <statement>
      <p permid="uKe">
        Are the statements <m>P \imp (Q\vee R)</m> and
        <m>(P \imp Q) \vee (P \imp R)</m> logically equivalent?
      </p>
    </statement>
      <!-- <solution>
        <p>
          Again, make two truth tables. The statements are logically equivalent.
        </p>
      </solution> -->
  </exercise>

  <exercise permid="zBb">
    <statement>
      <p permid="aRn">
        Simplify the following statements
        (so that negation only appears right before variables).

        <ol permid="UdM">
          <li permid="mRk"><m>\neg(P \imp \neg Q)</m>.</li>

          <li permid="SYt">
            <m>(\neg P \vee \neg Q) \imp \neg (\neg Q \wedge R)</m>.
          </li>

          <li permid="zfC">
            <m>\neg((P \imp \neg Q) \vee \neg (R \wedge \neg R))</m>.
          </li>

          <li permid="fmL">
            <p permid="wUQ">
              It is false that if Sam is not a man then Chris is a woman,
              and that Chris is not a woman.
            </p>
          </li>
        </ol>
      </p>
    </statement>
    <solution permid="mhq">
      <p permid="Ush">
        <ol permid="PtT">
          <li permid="LtU"><m>P \wedge Q</m>.</li>

          <li permid="rBd">
            <m>(\neg P \vee \neg R) \imp (Q \vee \neg R)</m> or,
            replacing the implication with a disjunction first:
            <m>(P \wedge Q) \vee (Q \vee \neg R)</m>.
          </li>

          <li permid="XIm">
            <p permid="dbZ">
              <m>(P \wedge Q) \wedge (R \wedge \neg R)</m>.
              This is necessarily false,
              so it is also equivalent to <m>P \wedge \neg P</m>.
            </p>
          </li>

          <li permid="DPv">
            <p permid="Jji">
              Either Sam is a woman and Chris is a man, or Chris is a woman.
            </p>
          </li>
        </ol>
      </p>
    </solution>
  </exercise>

  <exercise permid="fIk">
    <statement>
      <p permid="GYw">
        Use De Morgan's Laws,
        and any other logical equivalence facts you know to simplify the following statements.
        Show all your steps.
        Your final statements should have negations only appear directly next to the sentence variables or predicates (<m>P</m>,
        <m>Q</m>, <m>E(x)</m>, etc.), and no double negations.
        It would be a good idea to use only conjunctions,
        disjunctions, and negations.

        <ol permid="AkV">
          <li permid="jWE">
            <m>\neg((\neg P \wedge Q) \vee \neg(R \vee \neg S))</m>.
          </li>

          <li permid="QdN">
            <m>\neg((\neg P \imp \neg Q) \wedge (\neg Q \imp R))</m>
            (careful with the implications).
          </li>

          <li permid="wkW">
            <p permid="pqr">
              For both parts above,
              verify your answers are correct using truth tables.
              That is, use a truth table to check that the given statement and your proposed simplification are actually logically equivalent.
            </p>
          </li>
        </ol>
      </p>
    </statement>
    <solution permid="RIw" category="instructor">
      <p permid="vju">
        <ol permid="Czy">
          <li permid="KNR">
            <p permid="zjt">
              <m>\neg((\neg P \wedge Q) \vee \neg(R \vee \neg S))</m>
            </p>

            <p permid="fqC">
              <m>\neg(\neg P \wedge Q) \wedge \neg\neg(R \vee \neg S)</m> by De Morgan's law.
            </p>

            <p permid="LxL">
              <m>\neg(\neg P \wedge Q) \wedge (R \vee \neg S)</m> by double negation.
            </p>

            <p permid="rEU">
              <m>(\neg\neg P \vee \neg Q) \wedge (R \vee \neg S)</m> by De Morgan's law.
            </p>

            <p permid="XMd">
              <m>(P \vee \neg Q) \wedge (R \vee \neg S)</m> by double negation.
            </p>
          </li>

          <li permid="qVa">
            <p permid="DTm">
              We will need to convert the implications to disjunctions so we can apply De Morgan's law:
            </p>

            <p permid="kav">
              <m>\neg((\neg P \imp \neg Q) \wedge (\neg Q \imp R))</m>
            </p>

            <p permid="QhE">
              <m>\neg((\neg \neg P \vee \neg Q) \wedge (\neg\neg Q \vee R))</m> by implication/disjunction equivalence.
            </p>

            <p permid="woN">
              <m>\neg((P \vee \neg Q) \wedge (Q \vee R))</m> by double negation.
            </p>

            <p permid="cvW">
              <m>\neg(P \vee \neg Q) \vee \neg (Q \vee R)</m> by De Morgan's law.
            </p>

            <p permid="IDf">
              <m>(\neg P \wedge \neg \neg Q) \vee (\neg Q \wedge \neg R)</m> by De Morgan's law.
            </p>

            <p permid="oKo">
              <m>(\neg P \wedge Q) \vee (\neg Q \wedge \neg R)</m> by double negation.
            </p>
          </li>

          <li permid="Xcj">
            <p permid="URx">
              For each truth table,
              the columns for the original statement and the simplified statement must be identical.
              They are.
              For purposes of checking your work,
              here are the final columns for the two parts above:
            </p>

            <sidebyside permid="Jud" width="60%">

              <tabular permid="Lcm" halign="center">
                <row bottom="medium">
                  <cell right="medium"><m>P</m></cell>
                  <cell right="medium"><m>Q</m></cell>
                  <cell right="medium"><m>R</m></cell>
                  <cell right="medium">(a)</cell>
                  <cell>(b)</cell>
                </row>
                <row>
                  <cell right="medium">T</cell>
                  <cell right="medium">T</cell>
                  <cell right="medium">T</cell>
                  <cell right="medium">T</cell>
                  <cell>F</cell>
                </row>
                <row>
                  <cell right="medium">T</cell>
                  <cell right="medium">T</cell>
                  <cell right="medium">F</cell>
                  <cell right="medium">F</cell>
                  <cell>F</cell>
                </row>
                <row>
                  <cell right="medium">T</cell>
                  <cell right="medium">F</cell>
                  <cell right="medium">T</cell>
                  <cell right="medium">T</cell>
                  <cell>F</cell>
                </row>
                <row>
                  <cell right="medium">T</cell>
                  <cell right="medium">F</cell>
                  <cell right="medium">F</cell>
                  <cell right="medium">T</cell>
                  <cell>T</cell>
                </row>
                <row>
                  <cell right="medium">F</cell>
                  <cell right="medium">T</cell>
                  <cell right="medium">T</cell>
                  <cell right="medium">F</cell>
                  <cell>T</cell>
                </row>
                <row>
                  <cell right="medium">F</cell>
                  <cell right="medium">T</cell>
                  <cell right="medium">F</cell>
                  <cell right="medium">F</cell>
                  <cell>T</cell>
                </row>
                <row>
                  <cell right="medium">F</cell>
                  <cell right="medium">F</cell>
                  <cell right="medium">T</cell>
                  <cell right="medium">T</cell>
                  <cell>F</cell>
                </row>
                <row>
                  <cell right="medium">F</cell>
                  <cell right="medium">F</cell>
                  <cell right="medium">F</cell>
                  <cell right="medium">T</cell>
                  <cell>T</cell>
                </row>
              </tabular>

            </sidebyside>

          </li>
        </ol>
      </p>
    </solution>
  </exercise>

  <exercise permid="LPt">
    <statement>
      <p permid="nfF">
        Consider the statement,
        <q>If a number is triangular or square, then it is not prime</q>

        <ol permid="gse">
          <li permid="csf">
            <p permid="VxA">
              Make a truth table for the statement <m>(T \vee S) \imp \neg P</m>.
            </p>
          </li>

          <li permid="Izo">
            <p permid="BEJ">
              If you believed the statement was <em>false</em>,
              what properties would a counterexample need to possess?
              Explain by referencing your truth table.
            </p>
          </li>

          <li permid="oGx">
            <p permid="hLS">
              If the statement were true,
              what could you conclude about the number 5657, which is definitely prime?
              Again, explain using the truth table.
            </p>
          </li>
        </ol>
      </p>
    </statement>
    <hint permid="Soz">
      <p permid="Fjj">
        <ol permid="bIl">
          <li permid="UNG">
            <p permid="NTb">
              There will be three rows in which the statement is false.
            </p>
          </li>
          <li permid="AUP">
            <p permid="uak">
              Consider the three rows that evaluate to false and say what the truth values of <m>T</m>, <m>S</m>, and <m>P</m> are there.
            </p>
          </li>
          <li permid="hbY">
            <p permid="aht">
              You are looking for a row in which <m>P</m> is true, and the whole statement is true.
            </p>
          </li>
        </ol>
      </p>
    </hint>
    <solution category="instructor">
      <p>
        <ol>
          <li>

            <sidebyside width="50%">

              <tabular halign="center">
                <row bottom="medium">
                  <cell right="medium"><m>T</m></cell>
                  <cell right="medium"><m>S</m></cell>
                  <cell right="medium"><m>P</m></cell>
                  <cell><m>(T\vee S) \imp \neg P</m></cell>
                </row>
                <row>
                  <cell right="medium">T</cell>
                  <cell right="medium">T</cell>
                  <cell right="medium">T</cell>
                  <cell>F</cell>
                </row>
                <row>
                  <cell right="medium">T</cell>
                  <cell right="medium">T</cell>
                  <cell right="medium">F</cell>
                  <cell>T</cell>
                </row>
                <row>
                  <cell right="medium">T</cell>
                  <cell right="medium">F</cell>
                  <cell right="medium">T</cell>
                  <cell>F</cell>
                </row>
                <row>
                  <cell right="medium">T</cell>
                  <cell right="medium">F</cell>
                  <cell right="medium">F</cell>
                  <cell>T</cell>
                </row>
                <row>
                  <cell right="medium">F</cell>
                  <cell right="medium">T</cell>
                  <cell right="medium">T</cell>
                  <cell>F</cell>
                </row>
                <row>
                  <cell right="medium">F</cell>
                  <cell right="medium">T</cell>
                  <cell right="medium">F</cell>
                  <cell>T</cell>
                </row>
                <row>
                  <cell right="medium">F</cell>
                  <cell right="medium">F</cell>
                  <cell right="medium">T</cell>
                  <cell>T</cell>
                </row>
                <row>
                  <cell right="medium">F</cell>
                  <cell right="medium">F</cell>
                  <cell right="medium">F</cell>
                  <cell>T</cell>
                </row>
              </tabular>

            </sidebyside>

          </li>

          <li>
            <p>
              There are three cases in which the statement is false:
              rows 1, 3 and 5.
              So one way to prove this was false would be to find a number that was triangular,
              square and prime
              (row 1).
              Or you could find a number that was triangular, not square,
              and prime (row 3) or one that is not triangular,
              is square and is not prime
              (row 5).
              In fact, since no square number is prime,
              we would need to do the second one (3 is both triangular and prime,
              but in fact this is the only one).
            </p>
          </li>

          <li>
            <p>
              Here we have a prime number,
              so we need to look at rows in which <m>P</m> is true.
              We also need to statement to be true.
              There is only one row with both these properties: row 7.
              And here we see that <m>T</m> and <m>S</m> are both false.
              So we would know that 5657 is neither triangular nor square.
            </p>
          </li>
        </ol>
      </p>
    </solution>
  </exercise>

  <exercise permid="rWC">
    <statement>
      <p permid="TmO">
        Tommy Flanagan was telling you what he ate yesterday afternoon.
        He tells you, <q>I had either popcorn or raisins.
        Also, if I had cucumber sandwiches, then I had soda.
        But I didn't drink soda or tea.</q>
        Of course you know that Tommy is the worlds worst liar,
        and everything he says is false.
        What did Tommy eat?
      </p>

      <p permid="ztX">
        Justify your answer by writing all of Tommy's statements using sentence variables (<m>P, Q, R, S, T</m>),
        taking their negations, and using these to deduce what Tommy actually ate.
      </p>
    </statement>
    <hint permid="yvI">
      <p permid="lqs">
        Write down three statements, and then take the negation of each (since he is a liar).  You should find that Tommy ate one item and drank one item.  (<m>Q</m> is for cucumber sandwiches.)
      </p>
    </hint>
    <solution category="instructor">
      <p>
        Let <m>P</m> be the statement,
        <q>I had popcorn,</q> <m>Q</m> be the statement,
        <q>I had cucumber sandwiches,</q>
        <m>R</m> be the statement,
        <q>I had raisins,</q> <m>S</m> be,
        <q>I had soda,</q> and <m>T</m> be,
        <q>I had tea.</q> Then the statements made by Tommy are:
        <me>
          P \vee R \qquad Q \imp S \qquad \neg(S \vee T)
        </me>
      </p>

      <p>
        We need the negation of all of these.
        Thus what is true is:
        <me>
          \neg P \wedge \neg R \qquad Q \wedge \neg S \qquad S \vee T
        </me>
      </p>

      <p>
        From the first two statements we can conclude that Tommy did not eat popcorn,
        did not eat raisins,
        did eat cucumber sandwiches and did not drink soda.
        From the last statement <m>S \vee T</m> and the fact that we know <m>\neg S</m> we can conclude <m>T</m>,
        so Tommy did drink tea.
      </p>
    </solution>
  </exercise>

  <exercise permid="YdL">
    <statement>
      <p permid="fBg">
        Determine if the following deduction rule is valid:
      </p>

      <sidebyside permid="xLO">

        <tabular halign="center" permid="hqt">
          <row>
            <cell/>
            <cell><m>P \vee Q</m></cell>
          </row>
          <row bottom="minor">
            <cell/>
            <cell><m>\neg P</m></cell>
          </row>
          <row>
            <cell><m>\therefore</m></cell>
            <cell><m>Q</m></cell>
          </row>
        </tabular>

      </sidebyside>
    </statement>
    <solution permid="eCR">
      <p permid="Azq">
        The deduction rule is valid.
        To see this,
        make a truth table which contains <m>P \vee Q</m> and <m>\neg P</m>
        (and <m>P</m> and <m>Q</m> of course).
        Look at the truth value of <m>Q</m> in each of the rows that have
        <m>P \vee Q</m> and <m>\neg P</m> true.
      </p>
    </solution>
  </exercise>

  <exercise permid="EkU">
    <statement>
      <p permid="LIp">
        Determine if the following is a valid deduction rule:
      </p>

      <sidebyside permid="dSX">

        <tabular halign="center" permid="NxC">
          <row>
            <cell/>
            <cell><m>P \imp (Q \vee R)</m></cell>
          </row>
          <row bottom="minor">
            <cell/>
            <cell><m>\neg(P \imp Q)</m></cell>
          </row>
          <row>
            <cell><m>\therefore</m></cell>
            <cell><m>R</m></cell>
          </row>
        </tabular>

      </sidebyside>
    </statement>
      <!-- <solution>
        <p>
          The deduction rule is valid. Again, make a truth table containing the premises and conclusion. Look at the rows for which the premises are true.
        </p>
      </solution> -->
  </exercise>

  <exercise permid="ksd">
    <statement>
      <p permid="rPy">
        Determine if the following is a valid deduction rule:
      </p>

      <sidebyside permid="Kag">

        <tabular halign="center" permid="tEL">
          <row>
            <cell/>
            <cell><m>(P \wedge Q) \imp R</m></cell>
          </row>
          <row bottom="minor">
            <cell/>
            <cell><m>\neg P \vee \neg Q</m></cell>
          </row>
          <row>
            <cell><m>\therefore</m></cell>
            <cell><m>\neg R</m></cell>
          </row>
        </tabular>

      </sidebyside>
    </statement>
      <!-- <solution>
        <p>
          The rule is NOT valid. If you make a truth table containing the premises and conclusion, there will be a row with both premises true but the conclusion false. For example, if <m>P</m> and <m>Q</m> are false and <m>R</m> is true, then <m>P \wedge Q</m> is false, so <m>(P \wedge Q) \imp R</m> is true. Also <m>\neg P</m> is true, so <m>\neg P \vee \neg Q</m> is true. However, <m>\neg R</m> is false.
        </p>
      </solution> -->
  </exercise>

  <exercise permid="Qzm">
    <statement>
      <p permid="XWH">
        Can you chain implications together?
        That is, if <m>P \imp Q</m> and <m>Q \imp R</m>,
        does that means the <m>P \imp R</m>?
        Can you chain more implications together?
        Let's find out:

        <ol permid="Mzn">
          <li permid="Njh">
            <p permid="GoC">
              Prove that the following is a valid deduction rule:
            </p>

            <sidebyside permid="qhp">

              <tabular halign="center" permid="ZLU">
                <row>
                  <cell/>
                  <cell><m>P \imp Q</m></cell>
                </row>
                <row bottom="minor">
                  <cell/>
                  <cell><m>Q \imp R</m></cell>
                </row>
                <row>
                  <cell><m>\therefore</m></cell>
                  <cell><m>P \imp R</m></cell>
                </row>
              </tabular>

            </sidebyside>
            <!-- <solution>
              <p>
                Consider the truth table:
              </p>
              <tabular halign="center">
                <row>
                  <cell><m>P</m></cell>
                  <cell><m>Q</m></cell>
                  <cell><m>R</m></cell>
                  <cell><m>P\imp Q</m></cell>
                  <cell><m>Q \imp R</m></cell>
                  <cell><m>P \imp R</m></cell>
                </row>
                <row bottom="minor">
                  <cell></cell>
                  <cell></cell>
                  <cell></cell>
                  <cell></cell>
                  <cell></cell>
                  <cell></cell>
                </row>
                <row>
                  <cell>T</cell>
                  <cell>T</cell>
                  <cell>T</cell>
                  <cell>T</cell>
                  <cell>T</cell>
                  <cell>T</cell>
                </row>
                <row>
                  <cell>T</cell>
                  <cell>T</cell>
                  <cell>F</cell>
                  <cell>T</cell>
                  <cell>F</cell>
                  <cell>F</cell>
                </row>
                <row>
                  <cell>T</cell>
                  <cell>F</cell>
                  <cell>T</cell>
                  <cell>F</cell>
                  <cell>T</cell>
                  <cell>T</cell>
                </row>
                <row>
                  <cell>T</cell>
                  <cell>F</cell>
                  <cell>F</cell>
                  <cell>F</cell>
                  <cell>T</cell>
                  <cell>F</cell>
                </row>
                <row>
                  <cell>F</cell>
                  <cell>T</cell>
                  <cell>T</cell>
                  <cell>T</cell>
                  <cell>T</cell>
                  <cell>T</cell>
                </row>
                <row>
                  <cell>F</cell>
                  <cell>T</cell>
                  <cell>F</cell>
                  <cell>T</cell>
                  <cell>F</cell>
                  <cell>T</cell>
                </row>
                <row>
                  <cell>F</cell>
                  <cell>F</cell>
                  <cell>T</cell>
                  <cell>T</cell>
                  <cell>T</cell>
                  <cell>T</cell>
                </row>
                <row>
                  <cell>F</cell>
                  <cell>F</cell>
                  <cell>F</cell>
                  <cell>T</cell>
                  <cell>T</cell>
                  <cell>T</cell>
                </row>
                <row>
                  <cell></cell>
                </row>
              </tabular>
              <p>
                Notice that both <m>P \imp Q</m> and <m>Q \imp R</m> are true in rows 1, 5, 7 and 8. In each of these rows, <m>P \imp R</m> is also true. So whenever the premises are true, so in the conclusion. Thus the deduction rule is valid.
              </p>
            </solution> -->
          </li>

          <li permid="tqq">
            <p permid="mvL">
              Prove that the following is a valid deduction rule for any <m>n \ge 2</m>:
            </p>

            <sidebyside permid="Woy">

              <tabular halign="center" permid="FTd">
                <row>
                  <cell/>
                  <cell><m>P_1 \imp P_2</m></cell>
                </row>
                <row>
                  <cell/>
                  <cell><m>P_2 \imp P_3</m></cell>
                </row>
                <row>
                  <cell/>
                  <cell><m>\vdots</m></cell>
                </row>
                <row bottom="minor">
                  <cell/>
                  <cell><m>P_{n-1} \imp P_n</m></cell>
                </row>
                <row>
                  <cell><m>\therefore</m></cell>
                  <cell><m>P_1 \imp P_n</m>.</cell>
                </row>
              </tabular>

            </sidebyside>

            <p permid="SCU">
              I suggest you don't go through the trouble of writing out a <m>2^n</m> row truth table.
              Instead, you should use part (a) and mathematical induction.
            <!-- <solution>
              <p>
                Part (a) is the inductive case. Now assume that the deduction rule holds going up to <m>P_k</m>. That is,
            </p>
              <tabular halign="center">
                <row>
                  <cell></cell>
                  <cell><m>P_1 \imp P_2</m></cell>
                </row>
                <row>
                  <cell></cell>
                  <cell><m>P_2 \imp P_3</m></cell>
                </row>
                <row>
                  <cell></cell>
                  <cell><m>\vdots</m></cell>
                </row>
                <row>
                  <cell></cell>
                  <cell><m>P_{k-1} \imp P_k</m></cell>
                </row>
                <row bottom="minor">
                  <cell></cell>
                  <cell></cell>
                </row>
                <row>
                  <cell><m>\therefore</m></cell>
                  <cell><m>P_1 \imp P_k</m>.</cell>
                </row>
              </tabular>
              <p>
                Now suppose we have
              </p>
              <tabular halign="center">
                <row>
                  <cell></cell>
                  <cell><m>P_1 \imp P_2</m></cell>
                </row>
                <row>
                  <cell></cell>
                  <cell><m>P_2 \imp P_3</m></cell>
                </row>
                <row>
                  <cell></cell>
                  <cell><m>\vdots</m></cell>
                </row>
                <row>
                  <cell></cell>
                  <cell><m>P_{k-1} \imp P_k</m></cell>
                </row>
                <row>
                  <cell></cell>
                  <cell><m>P_k \imp P_{k+1}</m></cell>
                </row>
              </tabular>
              <p>
                From the first <m>k-1</m> lines, we can conclude <m>P_1 \imp P_k</m>. The combining this with the last line, we can conclude (using part (a) again):
              </p>
              <tabular halign="center">
                <row>
                  <cell></cell>
                  <cell><m>P_1 \imp P_k</m></cell>
                </row>
                <row>
                  <cell></cell>
                  <cell><m>P_{k} \imp P_{k+1}</m></cell>
                </row>
                <row bottom="minor">
                  <cell></cell>
                  <cell></cell>
                </row>
                <row>
                  <cell><m>\therefore</m></cell>
                  <cell><m>P_1 \imp P_{k+1}</m>.</cell>
                </row>
              </tabular>
              <p>
                So
              </p>
              <tabular halign="center">
                <row>
                  <cell></cell>
                  <cell><m>P_1 \imp P_2</m></cell>
                </row>
                <row>
                  <cell></cell>
                  <cell><m>P_2 \imp P_3</m></cell>
                </row>
                <row>
                  <cell></cell>
                  <cell><m>\vdots</m></cell>
                </row>
                <row>
                  <cell></cell>
                  <cell><m>P_{k-1} \imp P_k</m></cell>
                </row>
                <row>
                  <cell></cell>
                  <cell><m>P_k \imp P_{k+1}</m></cell>
                </row>
                <row bottom="minor">
                  <cell></cell>
                  <cell></cell>
                </row>
                <row>
                  <cell><m>\therefore</m></cell>
                  <cell><m>P_1 \imp P_{k+1}</m>.</cell>
                </row>
              </tabular>
            </solution> -->
            </p>
          </li>
        </ol>
      </p>
    </statement>
    <hint permid="KKa">
      <p permid="RxB">
        For the second part, you can inductively assume that from the first <m>n-2</m> implications you can deduce <m>P_1 \imp P_{n-1}</m>.  Then you are back in the case in part (a) again.
      </p>
    </hint>
  </exercise>

  <exercise permid="wGv">
    <statement>
      <p permid="EdQ">
        We can also simplify statements in predicate logic using our rules for passing negations over quantifiers,
        and then applying propositional logical equivalence to the
        <q>inside</q> propositional part.
        Simplify the statements below
        (so negation appears only directly next to predicates).

        <ol permid="sGw">
          <li permid="Zxz">
            <m>\neg \exists x \forall y (\neg O(x) \vee E(y))</m>.
          </li>

          <li permid="FEI">
            <m>\neg \forall x \neg \forall y \neg(x \lt y \wedge \exists z (x \lt z \vee y \lt z))</m>.
          </li>

          <li permid="lLR">
            <p permid="yKd">
              There is a number <m>n</m> for which no other number is either less <m>n</m> than or equal to <m>n</m>.
            </p>
          </li>

          <li permid="RTa">
            <p permid="eRm">
              It is false that for every number <m>n</m> there are two other numbers which <m>n</m> is between.
            </p>
          </li>
        </ol>
      </p>
    </statement>
    <solution permid="qRj">
      <p permid="gGz">
        <ol permid="vBc">
          <li permid="yaj">
            <m>\forall x \exists y (O(x) \wedge \neg E(y))</m>.
          </li>

          <li permid="ehs">
            <m>\exists x \forall y (x \ge y \vee \forall z (x \ge z \wedge y \ge z))</m>.
          </li>

          <li permid="KoB">
            <p permid="KYv">
              There is a number <m>n</m> for which every other number is strictly greater than <m>n</m>.
            </p>
          </li>

          <li permid="qvK">
            <p permid="rfE">
              There is a number <m>n</m> which is not between any other two numbers.
            </p>
          </li>
        </ol>
      </p>
    </solution>
  </exercise>
  
  <exercise permid="cNE">
    <statement>
      <p permid="kkZ">
        Simplify the statements below to the point that negation symbols occur only directly next to predicates.
        <ol permid="YNF">
          <li permid="WCT">
            <p permid="XmN">
              <m>\neg \forall x \forall y (x \lt y \vee y \lt x)</m>.
            </p>
          </li>
          <li permid="CKc">
            <p permid="DtW">
              <m>\neg(\exists x P(x) \imp \forall y P(y))</m>.
            </p>
          </li>
        </ol>
      </p>
    </statement>
  </exercise>
  
  
  <exercise permid="IUN">
    <statement>
      <p permid="Qsi">
        Simplifying negations will be especially useful in the next section when we try to prove a statement by considering what would happen if it were false.  For each statement below, write the <em>negation</em> of the statement as simply as possible.  Don't just say, <q>it is false that <ellipsis/></q>.
        <ol permid="EUO">
          <li permid="iRl">
            <p permid="jBf">
              Every number is either even or odd.
            </p>
          </li>
          <li permid="OYu">
            <p permid="PIo">
              There is a sequence that is both arithmetic and geometric.
            </p>
          </li>
          <li permid="vfD">
            <p permid="vPx">
              For all numbers <m>n</m>, if <m>n</m> is prime, then <m>n+3</m> is not prime.
            </p>
          </li>
        </ol>
      </p>
    </statement>
    <hint permid="WYs">
      <p permid="xEK">
        It might help to translate the statements into symbols and then use the formulaic rules to simplify negations (i.e., rules for quantifiers and De Morgan's laws).  After simplifying, you should get <m>\forall x(\neg E(x) \wedge \neg O(x))</m>, for the first one, for example.  Then translate this back into English.
      </p>
    </hint>
  </exercise>
  

  <exercise permid="pbW">
    <statement>
      <p permid="wzr">
        Suppose <m>P</m> and <m>Q</m> are
        (possibly molecular)
        propositional statements.
        Prove that <m>P</m> and <m>Q</m> are logically equivalent if any only if <m>P \iff Q</m> is a tautology.
      </p>
    </statement>
    <hint permid="DfB">
      <p permid="dLT">
        What do these concepts mean in terms of truth tables?
      </p>
    </hint>
      <!-- TODO: needs solution -->
  </exercise>

  <exercise permid="Vjf">
    <statement>
      <p permid="cGA">
        Suppose <m>P_1, P_2, \ldots, P_n</m> and <m>Q</m> are
        (possibly molecular)
        propositional statements.
        Suppose further that
      </p>

      <sidebyside permid="CvH">

        <tabular permid="mam">
          <row>
            <cell/>
            <cell><m>P_1</m></cell>
          </row>
          <row>
            <cell/>
            <cell><m>P_2</m></cell>
          </row>
          <row>
            <cell/>
            <cell><m>\vdots</m></cell>
          </row>
          <row bottom="minor">
            <cell/>
            <cell><m>P_n</m></cell>
          </row>
          <row>
            <cell><m>\therefore</m></cell>
            <cell><m>Q</m></cell>
          </row>
        </tabular>

      </sidebyside>

      <p permid="INJ">
        is a valid deduction rule.
        Prove that the statement
        <me permid="oUS">
          (P_1 \wedge P_2 \wedge \cdots \wedge P_n) \imp Q
        </me>
        is a tautology.
      </p>
    </statement>
      <!-- TODO: needs solution -->
  </exercise>

</exercises>
